Fix pervasive off-by-one error in sprint length
I had previously defined 'sprint' so that the maximum length was 2p.
After carefully reviewing the original paper I discovered that I had
made an off-by-one error and that the actual maximum length should be
set at 2p+1.

The confusion comes from the fact that (in the relevant section of the
paper) 'n' refers to the *index* of the last element of the sprint, not
the *length* of the sprint. So when the paper states that n <= 2p it is
easy to misread that as setting the maximum sprint length to 2p, rather
than 2p+1.

With the previous definition it was possible to have a sprint of zero
length, but not with the new definition. Previously, many (nearly all)
theorems in Sprint.lean and Runner.lean needed to either prove that a
sprint was non-nil, or take a statement to that effect as an argument.
Since all sprints are non-nil now, we can remove these requirements.
The upside is that this should simplify things going forward. The
downside is that this change is much longer than it otherwise would be
as a result!

AngelDevil/Runner.lean
@@ -32,7 +32,6 @@ structure RunBuilder (p : Nat) where
   sprints : List (List RunState)
   -- These bundled properties are somewhat eclectic
   -- They are only included to facilitate the definition of 'extend_run' (below)
-  ppos : 0 < p
   nonnil : ∀ s ∈ sprints, s ≠ []
   samelen : steps A = sprints.length
   origin : (snn : sprints ≠ []) →
@@ -101,19 +100,16 @@ def next_sprint {p : Nat} (S : RunBuilder p) : List RunState :=
 
 lemma next_sprint_nonnil {p : Nat} (S : RunBuilder p) :
   next_sprint S ≠ [] := by
-  apply sprint_nonnil_of_ppos
-  exact S.ppos
+  exact sprint_nonnil _ _ _
 
 -- The initial state of the next sprint is the
 -- same as the final state of the builder
 lemma next_sprint_first_eq_builder_last {p : Nat} (S : RunBuilder p) :
   final_state S = (next_sprint S)[0]'(by
     apply List.length_pos_of_ne_nil
-    exact sprint_nonnil_of_ppos p (final_state S) _ S.ppos
+    exact next_sprint_nonnil _
   ) := by
-  unfold next_sprint
-  rw [sprint_getElem_zero_of_ppos]
-  exact S.ppos
+  exact (sprint_getElem_zero _ _ _).symm
 
 -- Every element of 'next_sprint' is close to its head
 lemma next_sprint_close_mem_head {p : Nat} (S : RunBuilder p) :
@@ -121,8 +117,7 @@ lemma next_sprint_close_mem_head {p : Nat} (S : RunBuilder p) :
   close p (loc x) (loc ((next_sprint S).head (next_sprint_nonnil _))) := by
   intro x xmem
   apply sprint_close_mem_head
-  · exact S.ppos
-  · exact xmem
+  exact xmem
 
 -- The last cell of the next sprint is "close" to the
 -- last cell of the builder journey.
@@ -130,38 +125,37 @@ lemma next_sprint_last_close_builder_last {p : Nat} (S : RunBuilder p) :
   close p (loc ((next_sprint S).getLast (next_sprint_nonnil _))) (last S.A) := by
   rw [← final_state_loc_eq_journey_last, next_sprint_first_eq_builder_last S]
   rw [close_comm, List.getElem_zero]
-  exact sprint_close_first_last _ S.ppos _ _
+  exact sprint_close_first_last _ _ _
 
 -- Define the base case for our builder construction:
 -- The journey has no steps, there are no sprints, and the
 -- Devil has only eaten one cell
-def empty_builder (D : Devil) (p : Nat) (ppos : 0 < p) : RunBuilder p where
+def empty_builder (D : Devil) (p : Nat) : RunBuilder p where
   D := D
   A := NoSteps p
   eaten := [response D (NoSteps p)]
   sprints := []
   nonnil := fun _ hs ↦ False.elim (List.not_mem_nil hs)
-  ppos := ppos
   samelen := by rw [nosteps_steps, List.length_nil]
   origin := fun snn ↦ False.elim (snn rfl)
   dest := fun snn ↦ False.elim (snn rfl)
 
-lemma empty_builder_sprints (D : Devil) (p : Nat) (ppos : 0 < p) :
-  (empty_builder D p ppos).sprints = [] := by
+lemma empty_builder_sprints (D : Devil) (p : Nat) :
+  (empty_builder D p).sprints = [] := by
   unfold empty_builder; dsimp
 
-lemma empty_builder_journey (D : Devil) (p : Nat) (ppos : 0 < p) :
-  (empty_builder D p ppos).A = NoSteps p := by
+lemma empty_builder_journey (D : Devil) (p : Nat) :
+  (empty_builder D p).A = NoSteps p := by
   unfold empty_builder; dsimp
 
-lemma empty_builder_eaten (D : Devil) (p : Nat) (ppos : 0 < p) :
-  (empty_builder D p ppos).eaten = [response D (NoSteps p)] := by
+lemma empty_builder_eaten (D : Devil) (p : Nat) :
+  (empty_builder D p).eaten = [response D (NoSteps p)] := by
   unfold empty_builder; dsimp
 
 -- Construct the journey that corresponds to appending the
 -- last location of the next sprint
 def builder_journey_extend {p : Nat} (S : RunBuilder p) : Journey p :=
-  append_journey S.A (loc ((next_sprint S).getLast (sprint_nonnil_of_ppos p _ _ S.ppos)))
+  append_journey S.A (loc ((next_sprint S).getLast (sprint_nonnil p _ _)))
   ((close_comm p _ _).mp (next_sprint_last_close_builder_last S))
 
 -- Why doesn't this theorem aleady exist?
@@ -176,17 +170,16 @@ lemma list_singleton_ne_nil {α : Type} (x : α) : [x] ≠ [] := by
    directly construct the RunBuilder (rather than taking 'S' as an argument).
    Unfortunately this caused timeouts, so now 'make_run' handles the recursion
    separately and wraps 'extend_run' -/
-def extend_run (D : Devil) (p : Nat) (ppos : 0 < p) (S : RunBuilder p) : RunBuilder p:=
+def extend_run (D : Devil) (p : Nat) (S : RunBuilder p) : RunBuilder p:=
   RunBuilder.mk D
     (builder_journey_extend S)
     (S.eaten ++ [response D (builder_journey_extend S)])
     (S.sprints ++ [next_sprint S])
-    ppos
     (by
       intro s smem
       rcases List.mem_append.mp smem with lhs | rhs
       · exact RunBuilder.nonnil _ s lhs
-      · exact (List.mem_singleton.mp rhs) ▸ (sprint_nonnil_of_ppos p _ _ ppos)
+      · exact (List.mem_singleton.mp rhs) ▸ (sprint_nonnil _ _ _)
     )
     (by
       unfold builder_journey_extend
@@ -221,50 +214,50 @@ def extend_run (D : Devil) (p : Nat) (ppos : 0 < p) (S : RunBuilder p) : RunBuil
     )
 
 -- Recursively construct the RunBuilder
-def make_run (D : Devil) (p n : Nat) (ppos : 0 < p) : RunBuilder p :=
-  if n = 0 then empty_builder D p ppos else
-  extend_run D p ppos (make_run D p (n - 1) ppos)
+def make_run (D : Devil) (p n : Nat) : RunBuilder p :=
+  if n = 0 then empty_builder D p else
+  extend_run D p (make_run D p (n - 1))
 
 -- A run of length zero is represented by the 'empty_builder'
-lemma make_run_eq_empty_of_length_zero (D : Devil) (p : Nat) (ppos : 0 < p) :
-  make_run D p 0 ppos = empty_builder D p ppos := by
+lemma make_run_eq_empty_of_length_zero (D : Devil) (p : Nat) :
+  make_run D p 0 = empty_builder D p := by
   unfold make_run
   rw [if_pos rfl]
 
 -- The recursive definition of the runner's journey:
 -- Append the last cell of the 'next_sprint' to the journey to extend it.
-lemma make_run_journey_recurrence (D : Devil) (p n : Nat) (ppos : 0 < p) (npos : 0 < n) :
-  (make_run D p n ppos).A =
+lemma make_run_journey_recurrence (D : Devil) (p n : Nat) (npos : 0 < n) :
+  (make_run D p n).A =
   append_journey
-    (make_run D p (n - 1) ppos).A
-    (loc ((next_sprint (make_run D p (n - 1) ppos)).getLast (sprint_nonnil_of_ppos p _ _ ppos)))
-    ((close_comm p _ _).mp (next_sprint_last_close_builder_last (make_run D p (n - 1) ppos))) := by
+    (make_run D p (n - 1)).A
+    (loc ((next_sprint (make_run D p (n - 1))).getLast (sprint_nonnil p _ _)))
+    ((close_comm p _ _).mp (next_sprint_last_close_builder_last (make_run D p (n - 1)))) := by
   nth_rw 1 [make_run]
   rw [if_neg (Nat.ne_zero_iff_zero_lt.mpr npos)]
   rfl
 
 -- The recursive definition of the runner's sprints
 -- Just append the 'next_sprint' to the existing list of sprints.
-lemma make_run_sprints_recurrence (D : Devil) (p n : Nat) (ppos : 0 < p) (npos : 0 < n) :
-  (make_run D p n ppos).sprints =
-  (make_run D p (n - 1) ppos).sprints ++ [(next_sprint (make_run D p (n - 1) ppos))] := by
+lemma make_run_sprints_recurrence (D : Devil) (p n : Nat) (npos : 0 < n) :
+  (make_run D p n).sprints =
+  (make_run D p (n - 1)).sprints ++ [(next_sprint (make_run D p (n - 1)))] := by
   nth_rw 1 [make_run]
   rw [if_neg (Nat.ne_zero_iff_zero_lt.mpr npos)]
   rfl
 
 -- The recursive definition of the cells eaten in response to the runner
 -- This is just the devil's response to the new journey append to the old list
-lemma make_run_eaten_recurrence (D : Devil) (p n : Nat) (ppos : 0 < p) (npos : 0 < n) :
-  (make_run D p n ppos).eaten =
-  (make_run D p (n - 1) ppos).eaten ++ [response D (make_run D p n ppos).A] := by
+lemma make_run_eaten_recurrence (D : Devil) (p n : Nat) (npos : 0 < n) :
+  (make_run D p n).eaten =
+  (make_run D p (n - 1)).eaten ++ [response D (make_run D p n).A] := by
   nth_rw 1 [make_run]
   rw [if_neg (Nat.ne_zero_iff_zero_lt.mpr npos)]
-  rw [make_run_journey_recurrence D p n ppos npos];
+  rw [make_run_journey_recurrence D p n npos];
   rfl
 
 -- The number of steps in the journey is just 'n'
-lemma make_run_journey_steps (D : Devil) (p n : Nat) (ppos : 0 < p) :
-  steps (make_run D p n ppos).A = n := by
+lemma make_run_journey_steps (D : Devil) (p n : Nat) :
+  steps (make_run D p n).A = n := by
   by_cases hnz : n = 0
   · subst hnz
     rw [make_run_eq_empty_of_length_zero, empty_builder_journey, nosteps_steps]
@@ -273,30 +266,30 @@ lemma make_run_journey_steps (D : Devil) (p n : Nat) (ppos : 0 < p) :
   rwa [make_run_journey_recurrence, append_steps, make_run_journey_steps, Nat.sub_one_add_one hnnz]
 
 -- The number of eaten cells is just n+1
-lemma make_run_eaten_length (D : Devil) (p n : Nat) (ppos : 0 < p) :
-  (make_run D p n ppos).eaten.length = n + 1 := by
+lemma make_run_eaten_length (D : Devil) (p n : Nat) :
+  (make_run D p n).eaten.length = n + 1 := by
   by_cases hnz : n = 0
   · subst hnz
     rw [make_run_eq_empty_of_length_zero, empty_builder_eaten, List.length_singleton]
   rename' hnz => hnnz; push_neg at hnnz
   have npos : 0 < n := Nat.ne_zero_iff_zero_lt.mp hnnz
-  rw [make_run_eaten_recurrence D p n ppos npos, List.length_append]
+  rw [make_run_eaten_recurrence D p n npos, List.length_append]
   rw [List.length_singleton]
   apply Nat.add_one_inj.mpr
   nth_rw 2 [← Nat.sub_one_add_one hnnz]
-  exact make_run_eaten_length D p (n - 1) ppos
+  exact make_run_eaten_length D p (n - 1)
 
 -- The number of sprints in the RunBuilder is 'n'
-lemma make_run_sprints_length (D : Devil) (p n : Nat) (ppos : 0 < p) :
-  (make_run D p n ppos).sprints.length = n := by
-  rw [← (make_run D p n ppos).samelen]
-  exact make_run_journey_steps _ _ _ _
+lemma make_run_sprints_length (D : Devil) (p n : Nat) :
+  (make_run D p n).sprints.length = n := by
+  rw [← (make_run D p n).samelen]
+  exact make_run_journey_steps _ _ _
 
 -- The subjourney of a 'make_run' journey is just the
 -- 'make_run' journey of that length
-lemma make_run_subjourney (D : Devil) (p m n : Nat) (ppos : 0 < p) (mlt : m < n + 1) :
-  subjourney (make_run D p n ppos).A m (by rwa [make_run_journey_steps]) =
-  (make_run D p m ppos).A := by
+lemma make_run_subjourney (D : Devil) (p m n : Nat) (mlt : m < n + 1) :
+  subjourney (make_run D p n).A m (by rwa [make_run_journey_steps]) =
+  (make_run D p m).A := by
   -- First handle the case where m = n
   by_cases hmn : m = n
   · subst hmn
@@ -309,21 +302,21 @@ lemma make_run_subjourney (D : Devil) (p m n : Nat) (ppos : 0 < p) (mlt : m < n 
   -- Prove a tighter bound on m
   have mlt' : m < n :=
     lt_of_le_of_ne (Nat.le_of_lt_add_one mlt) hmn
-  have hrecurse := make_run_journey_recurrence D p n ppos (Nat.pos_of_ne_zero nnz)
+  have hrecurse := make_run_journey_recurrence D p n (Nat.pos_of_ne_zero nnz)
   rw [subjourney_congr_journey hrecurse, append_subjourney]
   · -- Do the recursion
-    exact make_run_subjourney D p m (n - 1) ppos (by rwa [Nat.sub_one_add_one nnz])
+    exact make_run_subjourney D p m (n - 1) (by rwa [Nat.sub_one_add_one nnz])
 
 -- The first 'm+1' cells eaten in response to the runner moving 'n' steps
 -- will correspond to all the cells eaten in response to the runner moving
 -- 'm' steps.
-lemma make_run_eaten_take (D : Devil) (p m n : Nat) (ppos : 0 < p) (mlt : m < n + 1) :
-  (make_run D p n ppos).eaten.take (m+1) = (make_run D p m ppos).eaten := by
+lemma make_run_eaten_take (D : Devil) (p m n : Nat) (mlt : m < n + 1) :
+  (make_run D p n).eaten.take (m+1) = (make_run D p m).eaten := by
   -- First handle the case where m = n
   by_cases hmn : m = n
   · subst hmn
     convert List.take_length
-    exact (make_run_eaten_length D p m ppos).symm
+    exact (make_run_eaten_length D p m).symm
   push_neg at hmn
   -- If m ≠ n, n ≠ 0
   have nnz : n ≠ 0 :=
@@ -331,23 +324,23 @@ lemma make_run_eaten_take (D : Devil) (p m n : Nat) (ppos : 0 < p) (mlt : m < n 
   -- Prove a tighter bound on m
   have mlt' : m < n :=
     lt_of_le_of_ne (Nat.le_of_lt_add_one mlt) hmn
-  have hrecurse := make_run_eaten_recurrence D p n ppos (Nat.pos_of_ne_zero nnz)
+  have hrecurse := make_run_eaten_recurrence D p n (Nat.pos_of_ne_zero nnz)
   rw [hrecurse, List.take_append_of_le_length]
   · -- Do the recursion
-    exact make_run_eaten_take D p m (n - 1) ppos (by rwa [Nat.sub_one_add_one nnz])
+    exact make_run_eaten_take D p m (n - 1) (by rwa [Nat.sub_one_add_one nnz])
   -- Prove the remaining bounds check
   rw [make_run_eaten_length, Nat.sub_one_add_one nnz]
   exact Nat.add_one_le_of_lt mlt'
 
 -- The first 'm' sprints of a run of 'n' sprints are the same as
 -- the full list of sprints in a run of 'm' sprints
-lemma make_run_sprints_take (D : Devil) (p m n : Nat) (ppos : 0 < p) (mlt : m < n + 1) :
-  (make_run D p n ppos).sprints.take m = (make_run D p m ppos).sprints := by
+lemma make_run_sprints_take (D : Devil) (p m n : Nat) (mlt : m < n + 1) :
+  (make_run D p n).sprints.take m = (make_run D p m).sprints := by
   -- First handle the case where m = n
   by_cases hmn : m = n
   · subst hmn
     convert List.take_length
-    exact (make_run_sprints_length D p m ppos).symm
+    exact (make_run_sprints_length D p m).symm
   push_neg at hmn
   -- If m ≠ n, n ≠ 0
   have nnz : n ≠ 0 :=
@@ -355,10 +348,10 @@ lemma make_run_sprints_take (D : Devil) (p m n : Nat) (ppos : 0 < p) (mlt : m < 
   -- Prove a tighter bound on m
   have mlt' : m < n :=
     lt_of_le_of_ne (Nat.le_of_lt_add_one mlt) hmn
-  have hrecurse := make_run_sprints_recurrence D p n ppos (Nat.pos_of_ne_zero nnz)
+  have hrecurse := make_run_sprints_recurrence D p n (Nat.pos_of_ne_zero nnz)
   rw [hrecurse, List.take_append_of_le_length]
   · -- Do the recursion
-    exact make_run_sprints_take D p m (n - 1) ppos (by rwa [Nat.sub_one_add_one nnz])
+    exact make_run_sprints_take D p m (n - 1) (by rwa [Nat.sub_one_add_one nnz])
   -- Prove the remaining bounds check
   rw [make_run_sprints_length]
   apply Nat.le_of_lt_add_one
@@ -366,24 +359,24 @@ lemma make_run_sprints_take (D : Devil) (p m n : Nat) (ppos : 0 < p) (mlt : m < 
 
 -- Extract the runner's journey from the RunBuilder
 -- TODO: Is there any reason for this actually?
-def Runner (D : Devil) (p n : Nat) (ppos : 0 < p) : Journey p :=
-  (make_run D p n ppos).A
+def Runner (D : Devil) (p n : Nat) : Journey p :=
+  (make_run D p n).A
 
 -- Each cell in the runner's journey (other than the first)
 -- corresponds to the final location of the previous sprint.
-lemma make_run_journey_cell (D : Devil) (p n : Nat) (ppos : 0 < p) :
+lemma make_run_journey_cell (D : Devil) (p n : Nat) :
   ∀ i (ilt : i < n),
-  cell (make_run D p n ppos).A (i + 1)
+  cell (make_run D p n).A (i + 1)
     (by rw [make_run_journey_steps]; exact Nat.add_one_lt_add_one_iff.mpr ilt) =
-  (loc (((make_run D p n ppos).sprints[i]'
+  (loc (((make_run D p n).sprints[i]'
     (by rwa [make_run_sprints_length])).getLast
       (by
-        apply (make_run D p n ppos).nonnil
+        apply (make_run D p n).nonnil
         apply List.getElem_mem
       ))) := by
   intro i ilt
   -- Prove sprints is nonnil so we can use RunBuilder.dest below
-  have hsnn : (make_run D p (i + 1) ppos).sprints ≠ [] := by
+  have hsnn : (make_run D p (i + 1)).sprints ≠ [] := by
     apply List.ne_nil_of_length_pos
     rw [make_run_sprints_length]
     exact Nat.add_one_pos _
@@ -391,10 +384,10 @@ lemma make_run_journey_cell (D : Devil) (p n : Nat) (ppos : 0 < p) :
     Nat.add_one_lt_add_one_iff.mpr ilt
   rw [← subjourney_last_cell, make_run_subjourney]; swap
   · assumption -- bounds check
-  rw [((make_run D p (i + 1) ppos).dest hsnn).symm]
+  rw [((make_run D p (i + 1)).dest hsnn).symm]
   congr
   -- Rewrite the sprints of the sub-run as 'take' of the sprints of the full run.
-  rw [List.getLast_congr _ _ (make_run_sprints_take D p (i + 1) n ppos islt).symm]; swap
+  rw [List.getLast_congr _ _ (make_run_sprints_take D p (i + 1) n islt).symm]; swap
   · -- Resolve pending bounds check
     apply List.ne_nil_of_length_pos
     have ispos : 0 < i + 1 := Nat.add_one_pos _
@@ -409,16 +402,16 @@ lemma make_run_journey_cell (D : Devil) (p n : Nat) (ppos : 0 < p) :
     exact Nat.add_one_le_of_lt ilt
 
 -- Each cell in the 'eaten' list is the devil's response to some shorter journey
-lemma make_run_eaten (D : Devil) (p n : Nat) (ppos : 0 < p) :
+lemma make_run_eaten (D : Devil) (p n : Nat) :
   ∀ i (ilt : i < n + 1),
-  (make_run D p n ppos).eaten[i]'(by rwa [make_run_eaten_length]) =
-  (response D (make_run D p i ppos).A) := by
+  (make_run D p n).eaten[i]'(by rwa [make_run_eaten_length]) =
+  (response D (make_run D p i).A) := by
   intro i ilt
   -- If i ≠ n, we can recurse
   by_cases ilt' : i < n
   · have npos : 0 < n := Nat.zero_lt_of_lt ilt'
     have nnz : n ≠ 0 := Nat.ne_zero_of_lt npos
-    rw [getElem_congr_coll (make_run_eaten_recurrence D p n ppos npos)]
+    rw [getElem_congr_coll (make_run_eaten_recurrence D p n npos)]
     rw [← List.getElem_append_left']; swap
     · -- Resolve bounds check
       rwa [make_run_eaten_length, Nat.sub_one_add_one nnz]
@@ -430,54 +423,54 @@ lemma make_run_eaten (D : Devil) (p n : Nat) (ppos : 0 < p) :
   -- Handle the case where i = 0
   by_cases iz : i = 0
   · subst iz
-    have rwl : (make_run D p 0 ppos).eaten = [response D (NoSteps p)] := by
+    have rwl : (make_run D p 0).eaten = [response D (NoSteps p)] := by
       rw [make_run_eq_empty_of_length_zero, empty_builder_eaten]
-    have rwr : (make_run D p 0 ppos).A = (NoSteps p) := by
+    have rwr : (make_run D p 0).A = (NoSteps p) := by
       rw [make_run_eq_empty_of_length_zero, empty_builder_journey]
     rw [getElem_congr_coll rwl, rwr, List.getElem_singleton]
   rename' iz => inz; push_neg at inz
   have ipos : 0 < i := Nat.zero_lt_of_ne_zero inz
-  rw [getElem_congr_coll (make_run_eaten_recurrence D p i ppos ipos)]
+  rw [getElem_congr_coll (make_run_eaten_recurrence D p i ipos)]
   rw [List.getElem_append_right]; swap
   · -- Resolve bounds check
     rw [make_run_eaten_length, Nat.sub_one_add_one inz]
   rw [List.getElem_singleton]
 
 -- Each sprint is created by calling 'next_sprint' on some shorter 'make_run'
-lemma make_run_sprint (D : Devil) (p n : Nat) (ppos : 0 < p) :
+lemma make_run_sprint (D : Devil) (p n : Nat) :
   ∀ i (ilt : i < n),
-  (make_run D p n ppos).sprints[i]'(by rwa [make_run_sprints_length]) =
-  (next_sprint (make_run D p i ppos)) := by
+  (make_run D p n).sprints[i]'(by rwa [make_run_sprints_length]) =
+  (next_sprint (make_run D p i)) := by
   intro i ilt
-  rw [getElem_congr_coll (make_run_sprints_recurrence D p n ppos (Nat.zero_lt_of_lt ilt))]
+  rw [getElem_congr_coll (make_run_sprints_recurrence D p n (Nat.zero_lt_of_lt ilt))]
   by_cases ilt' : i < n - 1
   · rw [← List.getElem_append_left']; swap
     · rwa [make_run_sprints_length]
-    · convert make_run_sprint D p (n-1) ppos i ilt'
+    · convert make_run_sprint D p (n-1) i ilt'
   rename' ilt' => nple; push_neg at nple
   have inp := le_antisymm (Nat.le_sub_one_of_lt ilt) nple
   rw [List.getElem_append_right, List.getElem_singleton, inp]
   rwa [make_run_sprints_length]
 
 -- Every element of a sprint is close to the head of that sprint
-lemma make_run_close_sprint_mem_head (D : Devil) (p n : Nat) (ppos : 0 < p) :
-  ∀ s, (smem : s ∈ (make_run D p n ppos).sprints) → ∀ x ∈ s,
+lemma make_run_close_sprint_mem_head (D : Devil) (p n : Nat) :
+  ∀ s, (smem : s ∈ (make_run D p n).sprints) → ∀ x ∈ s,
   close p (loc x) (loc (s.head (RunBuilder.nonnil _ _ smem))) := by
   intro s smem x xmem
   rcases List.getElem_of_mem smem with ⟨i, ilt, rfl⟩
   rw [make_run_sprints_length] at ilt
-  have nseq := make_run_sprint D p n ppos i ilt
-  convert next_sprint_close_mem_head (make_run D p i ppos) x (nseq ▸ xmem)
+  have nseq := make_run_sprint D p n i ilt
+  convert next_sprint_close_mem_head (make_run D p i) x (nseq ▸ xmem)
 
 -- The last element of each sprint equals the first element of the next
 -- TODO: This seems longer than it should need to be.
 -- Perhaps we're missing some useful 'sprints' theorems?
-lemma make_run_sprint_last_eq_sprint_head (D : Devil) (p n : Nat) (ppos : 0 < p) :
+lemma make_run_sprint_last_eq_sprint_head (D : Devil) (p n : Nat) :
   ∀ i (islt : i + 1 < n),
-  ((make_run D p n ppos).sprints[i]'(by
+  ((make_run D p n).sprints[i]'(by
     rw [make_run_sprints_length]; exact lt_trans (Nat.lt_add_one _) islt)).getLast
     (by apply RunBuilder.nonnil _ _ (List.getElem_mem _)) =
-  ((make_run D p n ppos).sprints[i+1]'(by rwa [make_run_sprints_length])).head
+  ((make_run D p n).sprints[i+1]'(by rwa [make_run_sprints_length])).head
     (by apply RunBuilder.nonnil _ _ (List.getElem_mem _)) := by
   intro i islt
   have nnz : n ≠ 0 := by
@@ -485,28 +478,28 @@ lemma make_run_sprint_last_eq_sprint_head (D : Devil) (p n : Nat) (ppos : 0 < p)
     exact (Nat.not_lt_zero _) islt
   -- If i + 1 ≠ n - 1, we can close the goal with recursion
   by_cases islt' : i + 1 < n - 1
-  · convert make_run_sprint_last_eq_sprint_head D p (n - 1) ppos i islt' using 2
+  · convert make_run_sprint_last_eq_sprint_head D p (n - 1) i islt' using 2
     repeat
-    rw [getElem_congr_coll (make_run_sprints_recurrence D p n ppos (Nat.pos_of_ne_zero nnz))]
+    rw [getElem_congr_coll (make_run_sprints_recurrence D p n (Nat.pos_of_ne_zero nnz))]
     rw [← List.getElem_append_left']
   rename' islt' => nple; push_neg at nple
   have iseq := le_antisymm (Nat.le_sub_one_of_lt islt) nple
   rw [List.head_eq_getElem]
-  rw [getElem_congr_coll (make_run_sprint D p n ppos (i+1) islt)]
+  rw [getElem_congr_coll (make_run_sprint D p n (i+1) islt)]
   rw [← next_sprint_first_eq_builder_last]
   unfold final_state
-  have lnz : (make_run D p (i + 1) ppos).sprints.length ≠ 0 := by
+  have lnz : (make_run D p (i + 1)).sprints.length ≠ 0 := by
     rw [make_run_sprints_length]
     exact Nat.add_one_ne_zero _
   rw [dif_neg lnz]; congr
-  have mrst := make_run_sprints_take D p (i + 1) n ppos (lt_trans islt (Nat.lt_add_one _))
+  have mrst := make_run_sprints_take D p (i + 1) n (lt_trans islt (Nat.lt_add_one _))
   rw [← List.getLast_congr _ _ mrst]; swap
   · -- Resolve nil check
     intro hnil
     rcases List.take_eq_nil_iff.mp hnil with lhs | rhs
     · exact (Nat.add_one_ne_zero _) lhs
     · apply nnz
-      rw [← make_run_sprints_length D p n ppos]
+      rw [← make_run_sprints_length D p n]
       exact List.length_eq_zero_iff.mpr rhs
   rw [List.getLast_eq_getElem, List.getElem_take]; congr
   rw [List.length_take_of_le, Nat.add_one_sub_one]
@@ -514,17 +507,17 @@ lemma make_run_sprint_last_eq_sprint_head (D : Devil) (p n : Nat) (ppos : 0 < p)
   exact le_of_lt islt
 
 -- Every element of a sprint is "close" to the corresponding journey cell
-lemma make_run_sprint_mem_journey_cell_close (D : Devil) (p n : Nat) (ppos : 0 < p) :
-  ∀ i (ilt : i < n), ∀ rs ∈ (make_run D p n ppos).sprints[i]'(by rwa [make_run_sprints_length]),
-  close p (loc rs) (cell (make_run D p n ppos).A i
+lemma make_run_sprint_mem_journey_cell_close (D : Devil) (p n : Nat) :
+  ∀ i (ilt : i < n), ∀ rs ∈ (make_run D p n).sprints[i]'(by rwa [make_run_sprints_length]),
+  close p (loc rs) (cell (make_run D p n).A i
     (by rw [make_run_journey_steps]; exact lt_trans ilt (Nat.lt_add_one _))) := by
   intro i ilt rs hmem
   -- First handle the case where i = 0
   by_cases iz : i = 0
   · subst iz
     rw [journey_start]
-    convert make_run_close_sprint_mem_head D p n ppos _ (List.getElem_mem _) rs hmem using 1
-    have hnnil : (make_run D p n ppos).sprints ≠ [] := by
+    convert make_run_close_sprint_mem_head D p n _ (List.getElem_mem _) rs hmem using 1
+    have hnnil : (make_run D p n).sprints ≠ [] := by
       apply List.ne_nil_of_length_pos
       rwa [make_run_sprints_length]
     rw [List.head_eq_getElem_zero, RunBuilder.origin _ hnnil]; rfl
@@ -533,40 +526,40 @@ lemma make_run_sprint_mem_journey_cell_close (D : Devil) (p n : Nat) (ppos : 0 <
   have iplt : i - 1 < n := by
     apply lt_of_le_of_lt _ ilt
     exact Nat.sub_le _ _
-  have := make_run_journey_cell D p n ppos (i-1) iplt
+  have := make_run_journey_cell D p n (i-1) iplt
   rw [cell_congr_idx _ (Nat.sub_one_add_one inz)] at this
   rw [this, make_run_sprint_last_eq_sprint_head]; swap
   · -- Resolve bounds check
     rwa [Nat.sub_one_add_one inz]
-  apply make_run_close_sprint_mem_head D p n ppos
+  apply make_run_close_sprint_mem_head D p n
   · apply List.getElem_mem
   · convert hmem
     exact Nat.sub_one_add_one inz
 
--- List of blocked cells used to generate 'next_sprint (make_run D p n ppos)'
-def make_block_list (D : Devil) (p n : Nat) (ppos : 0 < p) : List (Int × Int) :=
-  List.union (make_run D p n ppos).eaten (west_wall p (make_run D p n ppos).eaten.length)
+-- List of blocked cells used to generate 'next_sprint (make_run D p n)'
+def make_block_list (D : Devil) (p n : Nat) : List (Int × Int) :=
+  List.union (make_run D p n).eaten (west_wall p (make_run D p n).eaten.length)
 
 -- Expand the 'next_sprint' of a 'make_run' using 'make_block_list'
-lemma next_sprint_make_run_def (D : Devil) (p n : Nat) (ppos : 0 < p) :
-  next_sprint (make_run D p n ppos) =
-  sprint p (final_state (make_run D p n ppos)) (make_block_list D p n ppos) := rfl
+lemma next_sprint_make_run_def (D : Devil) (p n : Nat) :
+  next_sprint (make_run D p n) =
+  sprint p (final_state (make_run D p n)) (make_block_list D p n) := rfl
 
 /- Note that it *is* possible to force the runner to remain on a blocked cell
    if the devil is not nice. Technically, even with a devil that isn't nice,
    the runner can never be forced onto a 'wall' cell (cells with x = -1, 0 ≤ y)
    but that proof is more difficult and we're only concerned with nice devils
    for this section of the proof so we can make our work easier by assuming such. -/
-lemma make_run_next_sprint_avoids_blocked_of_nice (D : Devil) (p n : Nat) (ppos : 0 < p) (hnice : nice D p) :
-  ∀ rs ∈ next_sprint (make_run D p n ppos), (loc rs) ∉ make_block_list D p n ppos := by
+lemma make_run_next_sprint_avoids_blocked_of_nice (D : Devil) (p n : Nat) (hnice : nice D p) :
+  ∀ rs ∈ next_sprint (make_run D p n), (loc rs) ∉ make_block_list D p n := by
   intro rs rsmem lrsmem
   -- First handle the case where n = 0
   -- This mostly involves showing that the origin will never be on the block list
   by_cases nz : n = 0
   · subst nz
-    apply sprint_avoids_blocked p _ (make_block_list D p 0 ppos) _ rs rsmem lrsmem
+    apply sprint_avoids_blocked p _ (make_block_list D p 0) _ rs rsmem lrsmem
     rw [make_run_eq_empty_of_length_zero]
-    rw [final_state_of_sprints_nil _ (empty_builder_sprints D p ppos)]
+    rw [final_state_of_sprints_nil _ (empty_builder_sprints D p)]
     unfold run_start loc; dsimp
     intro omem
     -- We have two cases depending on whether rs is an eaten cell or wall cell
@@ -584,46 +577,46 @@ lemma make_run_next_sprint_avoids_blocked_of_nice (D : Devil) (p n : Nat) (ppos 
       dsimp at this
       linarith
   rename' nz => nnz; push_neg at nnz
-  have hsnnil : (make_run D p n ppos).sprints ≠ [] := by
+  have hsnnil : (make_run D p n).sprints ≠ [] := by
     apply List.ne_nil_of_length_pos
     rw [make_run_sprints_length]
     exact Nat.pos_of_ne_zero nnz
   rw [next_sprint_make_run_def] at rsmem
   -- Use recursion to show that the run has thus far avoided blocked cells
   -- This will be required in order to use 'sprint_avoids_blocked'
-  have hsafe : loc (final_state (make_run D p n ppos)) ∉ make_block_list D p (n - 1) ppos := by
+  have hsafe : loc (final_state (make_run D p n)) ∉ make_block_list D p (n - 1) := by
     apply make_run_next_sprint_avoids_blocked_of_nice
     · assumption
-    convert final_state_getLast_mem_of_nonnil (make_run D p n ppos) hsnnil
-    rw [List.getLast_congr _ _ (make_run_sprints_recurrence D p n ppos (Nat.pos_of_ne_zero nnz))]; swap
+    convert final_state_getLast_mem_of_nonnil (make_run D p n) hsnnil
+    rw [List.getLast_congr _ _ (make_run_sprints_recurrence D p n (Nat.pos_of_ne_zero nnz))]; swap
     · apply List.append_ne_nil_of_right_ne_nil
       exact list_singleton_ne_nil _
     rw [List.getLast_append_right (list_singleton_ne_nil _)]
     exact (List.getLast_singleton (list_singleton_ne_nil _)).symm
   -- Strengthen the statement of 'hsafe' by including the devil's last response and
   -- an extra 'p' cells in the west wall. This section constitutes the majority of the proof.
-  have hsafe' : loc (final_state (make_run D p n ppos)) ∉ make_block_list D p n ppos := by
+  have hsafe' : loc (final_state (make_run D p n)) ∉ make_block_list D p n := by
     intro lfsmem
     rcases List.mem_union_iff.mp lfsmem with lhs | rhs
     · -- Handle the case where the final state is on the 'eaten' list
       rcases List.getElem_of_mem lhs with ⟨i, ilt, hi⟩
       rw [make_run_eaten_length] at ilt
-      rw [getElem_congr_coll (make_run_eaten_recurrence D p n ppos (Nat.pos_of_ne_zero nnz))] at hi
+      rw [getElem_congr_coll (make_run_eaten_recurrence D p n (Nat.pos_of_ne_zero nnz))] at hi
       -- Handle the case where the final state was eaten last
       by_cases hin : i = n
       · rw [List.getElem_append_right] at hi; swap
         · rw [make_run_eaten_length, hin, Nat.sub_one_add_one nnz]
         -- Prove a bound needed for 'getElem_singleton'
-        have lt1 : i - (make_run D p (n - 1) ppos).eaten.length < 1 := by
+        have lt1 : i - (make_run D p (n - 1)).eaten.length < 1 := by
           rw [make_run_eaten_length, Nat.sub_one_add_one nnz, hin, Nat.sub_self]
           norm_num
         rw [List.getElem_singleton lt1, final_state_loc_eq_journey_last] at hi
         -- We will show that a journey cell is eaten, which is contradiction with 'hnice'
         apply not_nice_of_eats_journey_cell D p _ hnice
-        use (make_run D p n ppos).A, n, n, le_refl n
+        use (make_run D p n).A, n, n, le_refl n
         use (by rw [make_run_journey_steps]; exact Nat.lt_add_one _)
-        have hsj := subjourney_full (make_run D p n ppos).A
-        rw [subjourney_congr_idx _ (make_run_journey_steps D p n ppos)] at hsj
+        have hsj := subjourney_full (make_run D p n).A
+        rw [subjourney_congr_idx _ (make_run_journey_steps D p n)] at hsj
         rw [hsj]
         convert hi
         rw [last]
@@ -633,7 +626,7 @@ lemma make_run_next_sprint_avoids_blocked_of_nice (D : Devil) (p n : Nat) (ppos 
         -- If i ≠ n, we will show that the final state was on the old eaten list - a contradiction
         apply hsafe
         apply List.mem_union_iff.mpr; left
-        have ilt' : i < (make_run D p (n - 1) ppos).eaten.length := by
+        have ilt' : i < (make_run D p (n - 1)).eaten.length := by
           rw [make_run_eaten_length, Nat.sub_one_add_one nnz]
           exact lt_of_le_of_ne (Nat.le_of_lt_add_one ilt) inen
         rw [List.getElem_append_left ilt'] at hi
@@ -646,7 +639,7 @@ lemma make_run_next_sprint_avoids_blocked_of_nice (D : Devil) (p n : Nat) (ppos 
       -- Handle the case where 'i' is so large, it exceeds the bound proven in Bound.lean
       by_cases pni : p * n < i
       · apply (lt_self_iff_false n).mp
-        nth_rw 2 [← make_run_journey_steps D p n ppos]
+        nth_rw 2 [← make_run_journey_steps D p n]
         apply journey_lb _ _ (lt_of_lt_of_le pni (le_trans _ (le_max_right _ _)))
         simp
         rw [← (Prod.ext_iff.mp hi).2, List.getElem_range]
@@ -660,9 +653,9 @@ lemma make_run_next_sprint_avoids_blocked_of_nice (D : Devil) (p n : Nat) (ppos 
         rwa [make_run_eaten_length, Nat.sub_one_add_one nnz]
   exact sprint_avoids_blocked p _ _ hsafe' rs rsmem lrsmem
 
-lemma make_run_journey_allowed_of_nice (D : Devil) (p n : Nat) (ppos : 0 < p) (hnice : nice D p) :
-  allowed D (make_run D p n ppos).A := by
-  let MR := make_run D p n ppos
+lemma make_run_journey_allowed_of_nice (D : Devil) (p n : Nat) (hnice : nice D p) :
+  allowed D (make_run D p n).A := by
+  let MR := make_run D p n
   change allowed D MR.A
   unfold allowed
   intro i j ilt jlt
@@ -675,16 +668,16 @@ lemma make_run_journey_allowed_of_nice (D : Devil) (p n : Nat) (ppos : 0 < p) (h
   have nnez : n ≠ 0 := Nat.ne_zero_of_lt npos
   -- Re-write the left-hand side using the journey recurrence
   have lhs_rw : subjourney MR.A i (lt_trans ilt jlt) =
-    subjourney (make_run D p (n - 1) ppos).A i (by
+    subjourney (make_run D p (n - 1)).A i (by
       rwa [make_run_journey_steps, Nat.sub_one_add_one]
       exact Nat.ne_zero_of_lt ilt'
     ) := by
-    rw [subjourney_congr_journey (make_run_journey_recurrence D p n ppos npos)]
+    rw [subjourney_congr_journey (make_run_journey_recurrence D p n npos)]
     rw [append_subjourney]
   -- If j ≠ n we can recurse, so handle that case first
   by_cases hjnn : n ≠ j
   · -- Now apply the journey recurrence on the right and recurse
-    rw [lhs_rw, cell_congr_journey (make_run_journey_recurrence D p n ppos npos)]
+    rw [lhs_rw, cell_congr_journey (make_run_journey_recurrence D p n npos)]
     rw [append_cell_ne_last]; swap
     · rw [make_run_journey_steps, Nat.sub_one_add_one nnez]
       exact lt_of_le_of_ne (Nat.le_of_lt_add_one jlt') hjnn.symm
@@ -693,12 +686,12 @@ lemma make_run_journey_allowed_of_nice (D : Devil) (p n : Nat) (ppos : 0 < p) (h
     · exact ilt
   rename' hjnn => hjn; push_neg at hjn
   subst hjn
-  have last_exp := (final_state_loc_eq_journey_last (make_run D p n ppos)).symm
-  rw [last, ← cell_congr_idx _ (make_run_journey_steps D p n ppos).symm jlt] at last_exp
-  rw [last_exp, make_run_subjourney D p i n ppos (lt_trans ilt (Nat.lt_add_one _))]
+  have last_exp := (final_state_loc_eq_journey_last (make_run D p n)).symm
+  rw [last, ← cell_congr_idx _ (make_run_journey_steps D p n ).symm jlt] at last_exp
+  rw [last_exp, make_run_subjourney D p i n (lt_trans ilt (Nat.lt_add_one _))]
   intro h
-  let fs : RunState := final_state (make_run D p n ppos)
-  have lfsmem : loc fs ∈ (make_run D p (n - 1) ppos).eaten := by
+  let fs : RunState := final_state (make_run D p n)
+  have lfsmem : loc fs ∈ (make_run D p (n - 1)).eaten := by
     apply @List.mem_of_mem_take _ (i + 1)
     rw [make_run_eaten_take]; swap
     · rwa [Nat.sub_one_add_one nnez]
@@ -716,12 +709,12 @@ lemma make_run_journey_allowed_of_nice (D : Devil) (p n : Nat) (ppos : 0 < p) (h
     apply List.mem_append_right
     rw [h]
     exact List.mem_singleton_self _
-  apply make_run_next_sprint_avoids_blocked_of_nice D p (n - 1) ppos hnice fs _ _
-  · convert final_state_getLast_mem_of_nonnil (make_run D p n ppos) (by
+  apply make_run_next_sprint_avoids_blocked_of_nice D p (n - 1) hnice fs _ _
+  · convert final_state_getLast_mem_of_nonnil (make_run D p n) (by
       apply List.ne_nil_of_length_pos
       rwa [make_run_sprints_length]
     )
-    rw [List.getLast_congr _ _ (make_run_sprints_recurrence D p n ppos npos)]; swap
+    rw [List.getLast_congr _ _ (make_run_sprints_recurrence D p n npos)]; swap
     · apply List.ne_nil_of_length_pos
       rw [List.length_append, List.length_singleton]
       exact lt_of_le_of_lt (Nat.zero_le _) (Nat.lt_add_one _)
@@ -733,30 +726,30 @@ lemma make_run_journey_allowed_of_nice (D : Devil) (p n : Nat) (ppos : 0 < p) (h
 /- Construct the list of run states corresponding to the full route of the runner.
    Each sprint overlaps by one cell, so we need to remove the first state from all
    but the first sprint -/
-def RunPath (D : Devil) (p n : Nat) (ppos : 0 < p) : List RunState :=
-  if hlz : (make_run D p n ppos).sprints.length = 0 then [run_start] else
-  ((make_run D p n ppos).sprints.head (List.ne_nil_of_length_pos (Nat.pos_of_ne_zero hlz))) ++
-  (List.flatten (List.map List.tail (make_run D p n ppos).sprints.tail))
+def RunPath (D : Devil) (p n : Nat) : List RunState :=
+  if hlz : (make_run D p n).sprints.length = 0 then [run_start] else
+  ((make_run D p n).sprints.head (List.ne_nil_of_length_pos (Nat.pos_of_ne_zero hlz))) ++
+  (List.flatten (List.map List.tail (make_run D p n).sprints.tail))
 
 -- A RunPath of length zero is just the singleton list [run_start]
-lemma run_path_of_length_zero (D : Devil) (p : Nat) (ppos : 0 < p) :
-  RunPath D p 0 ppos = [run_start] := by
+lemma run_path_of_length_zero (D : Devil) (p : Nat) :
+  RunPath D p 0 = [run_start] := by
   unfold RunPath make_run
   rw [dif_pos]
   rw [if_pos rfl, empty_builder_sprints]
   exact List.length_nil
 
 -- Any run state in the 'run path' must exist in some sprint of the run builder
-lemma make_run_sprints_getElem_exists_of_run_path_mem (D : Devil) (p n : Nat) (ppos : 0 < p)
-  (npos : 0 < n) (rs : RunState) (hmem : rs ∈ RunPath D p n ppos) :
-  ∃ (i : Nat) (ilt : i < ((make_run D p n ppos).sprints.length)),
-  ∃ (j : Nat) (jlt : j < ((make_run D p n ppos).sprints[i].length)),
-  (make_run D p n ppos).sprints[i][j] = rs := by
+lemma make_run_sprints_getElem_exists_of_run_path_mem (D : Devil) (p n : Nat)
+  (npos : 0 < n) (rs : RunState) (hmem : rs ∈ RunPath D p n) :
+  ∃ (i : Nat) (ilt : i < ((make_run D p n).sprints.length)),
+  ∃ (j : Nat) (jlt : j < ((make_run D p n).sprints[i].length)),
+  (make_run D p n).sprints[i][j] = rs := by
   unfold RunPath at hmem
-  have hslnz : (make_run D p n ppos).sprints.length ≠ 0 := by
+  have hslnz : (make_run D p n).sprints.length ≠ 0 := by
     rw [make_run_sprints_length]
     exact Nat.ne_zero_iff_zero_lt.mpr npos
-  have hslpos : 0 < (make_run D p n ppos).sprints.length :=
+  have hslpos : 0 < (make_run D p n).sprints.length :=
     Nat.pos_of_ne_zero hslnz
   rw [dif_neg hslnz] at hmem
   rcases List.mem_append.mp hmem with lhs | rhs
@@ -776,38 +769,38 @@ lemma make_run_sprints_getElem_exists_of_run_path_mem (D : Devil) (p n : Nat) (p
   exact rselem
 
 -- Recursive definition of RunPath in terms of 'make_run' sprints
-lemma run_path_recurrence (D : Devil) (p n : Nat) (ppos : 0 < p) (npos : 0 < n) :
-  (RunPath D p n ppos) =
-  (RunPath D p (n - 1) ppos) ++ ((make_run D p n ppos).sprints.getLast
+lemma run_path_recurrence (D : Devil) (p n : Nat) (npos : 0 < n) :
+  (RunPath D p n) =
+  (RunPath D p (n - 1)) ++ ((make_run D p n).sprints.getLast
     (by
       apply List.ne_nil_of_length_pos
       rwa [make_run_sprints_length]
     )).tail := by
   unfold RunPath
   have hnz : n ≠ 0 := Nat.ne_zero_of_lt npos
-  have hlnz : (make_run D p n ppos).sprints.length ≠ 0 := by
+  have hlnz : (make_run D p n).sprints.length ≠ 0 := by
     rwa [make_run_sprints_length]
-  have hlpos : 0 < (make_run D p n ppos).sprints.length := by
+  have hlpos : 0 < (make_run D p n).sprints.length := by
     exact Nat.pos_of_ne_zero hlnz
   rw [dif_neg hlnz]
   -- Handle the case where n = 1
   by_cases n1 : n = 1
   · subst n1
-    have hlz : (make_run D p (1 - 1) ppos).sprints.length = 0 := by
+    have hlz : (make_run D p (1 - 1)).sprints.length = 0 := by
       rw [make_run_sprints_length]
     rw [dif_pos hlz]
-    have hstn : (make_run D p 1 ppos).sprints.tail = [] := by
+    have hstn : (make_run D p 1).sprints.tail = [] := by
       apply List.eq_nil_of_length_eq_zero
       rw [List.length_tail, make_run_sprints_length, Nat.sub_self]
     rw [hstn, List.map_nil, List.flatten_nil, List.append_nil, ← List.getElem_zero_eq_head]; swap
     · assumption
-    have gE0nn : (make_run D p 1 ppos).sprints[0] ≠ [] := by
-      apply (make_run D p 1 ppos).nonnil
+    have gE0nn : (make_run D p 1).sprints[0] ≠ [] := by
+      apply (make_run D p 1).nonnil
       apply List.getElem_mem
     rw [← List.head_cons_tail _ gE0nn, List.singleton_append, ← List.getElem_zero_eq_head]; swap
     · -- Resolve bounds check
       exact List.length_pos_of_ne_nil gE0nn
-    rw [(make_run D p 1 ppos).origin]; swap
+    rw [(make_run D p 1).origin]; swap
     · -- Resolve bounds check
       exact List.ne_nil_of_length_pos hlpos
     rw [List.getLast_eq_getElem]; congr 2
@@ -816,16 +809,16 @@ lemma run_path_recurrence (D : Devil) (p n : Nat) (ppos : 0 < p) (npos : 0 < n) 
   rename' n1 => nne1; push_neg at nne1
   have h1ltn : 1 < n := by
     exact Nat.lt_of_le_of_ne (Nat.add_one_le_of_lt (Nat.pos_of_ne_zero hnz)) nne1.symm
-  have hlnz' : (make_run D p (n - 1) ppos).sprints.length ≠ 0 := by
+  have hlnz' : (make_run D p (n - 1)).sprints.length ≠ 0 := by
     rw [make_run_sprints_length]
     exact Nat.sub_ne_zero_of_lt h1ltn
-  have hlpos' : 0 < (make_run D p (n - 1) ppos).sprints.length := by
+  have hlpos' : 0 < (make_run D p (n - 1)).sprints.length := by
     exact Nat.pos_of_ne_zero hlnz'
   -- First, manipulate each side of the equation so that the
   -- left-hand sides of the appends match, and we can 'congr'
   rw [dif_neg hlnz', List.append_assoc, ← List.getElem_zero_eq_head]; swap
   · assumption
-  have := make_run_sprints_recurrence D p n ppos (Nat.pos_of_ne_zero hnz)
+  have := make_run_sprints_recurrence D p n (Nat.pos_of_ne_zero hnz)
   rw [getElem_congr_coll this]
   rw [List.getElem_append_left, List.getElem_zero_eq_head]; swap
   · -- Resolve bounds check
@@ -837,32 +830,33 @@ lemma run_path_recurrence (D : Devil) (p n : Nat) (ppos : 0 < p) (npos : 0 < n) 
     apply List.ne_nil_of_length_pos
     exact Nat.pos_of_ne_zero hlnz'
   rw [List.flatten_append, List.flatten_singleton]; congr
-  rw [← make_run_sprint D p n ppos, List.getLast_eq_getElem]
+  rw [← make_run_sprint D p n, List.getLast_eq_getElem]
   · congr; rw [make_run_sprints_length]
   · exact Nat.sub_lt npos (by norm_num)
 
 -- A predicate to check if 'rs' is an element of a particular sprint.
 -- Argument is of type 'Fin (n - 1 + 1)' to make it compatible with
 -- '_find_last' which requires an argument of type Fin (m+1) for some 'm'.
-abbrev is_sprint_mem (D : Devil) (p n : Nat) (ppos : 0 < p)
+abbrev is_sprint_mem (D : Devil) (p n : Nat)
   (npos : 0 < n) (rs : RunState) : (i : Fin (n - 1 + 1)) → Prop :=
-  fun i ↦ (rs ∈ (make_run D p n ppos).sprints[i]'(by
+  fun i ↦ (rs ∈ (make_run D p n).sprints[i]'(by
     rw [make_run_sprints_length]
     convert i.2
     exact (Nat.sub_one_add_one (Nat.ne_zero_of_lt npos)).symm))
 
+-- TODO: So.... which proof were these for? We don't seem to use them.
 -- Returns the index of the last sprint of the 'make_run' of which 'rs' is an element
 -- For the proof
-def find_last_sprint_with_state (D : Devil) (p n : Nat) (ppos : 0 < p)
+def find_last_sprint_with_state (D : Devil) (p n : Nat)
   (npos : 0 < n) (rs : RunState) : Nat :=
-  (_find_last (is_sprint_mem D p n ppos npos rs)).val
+  (_find_last (is_sprint_mem D p n npos rs)).val
 
 -- Prove that 'rs' appears in no later sprint than the one
 -- found by 'find_last_sprint_with_state'
 lemma last_sprint_with_state_is_last (D : Devil) (p n : Nat)
-  (ppos : 0 < p) (npos : 0 < n) (rs : RunState) : ∀ (i : Nat) (ilt : i < n),
-  rs ∈ (make_run D p n ppos).sprints[i]'(by rwa [make_run_sprints_length]) →
-  i ≤ find_last_sprint_with_state D p n ppos npos rs := by
+  (npos : 0 < n) (rs : RunState) : ∀ (i : Nat) (ilt : i < n),
+  rs ∈ (make_run D p n).sprints[i]'(by rwa [make_run_sprints_length]) →
+  i ≤ find_last_sprint_with_state D p n npos rs := by
   intro i ilt hmem
   unfold find_last_sprint_with_state
   -- First, work around Fin awkwardness
@@ -877,42 +871,42 @@ lemma last_sprint_with_state_is_last (D : Devil) (p n : Nat)
 -- The return value of 'find_last_sprint_with_state' is
 -- less than the number of sprints in the 'make_run'
 lemma last_sprint_with_state_lt_length (D : Devil) (p n : Nat)
-  (ppos : 0 < p) (npos : 0 < n) (rs : RunState) :
-  find_last_sprint_with_state D p n ppos npos rs < (make_run D p n ppos).sprints.length := by
+  (npos : 0 < n) (rs : RunState) :
+  find_last_sprint_with_state D p n npos rs < (make_run D p n).sprints.length := by
   unfold find_last_sprint_with_state
   rw [make_run_sprints_length]
   apply lt_of_lt_of_eq _ (Nat.sub_one_add_one (Nat.ne_zero_of_lt npos))
-  exact (_find_last (is_sprint_mem D p n ppos npos rs)).2
+  exact (_find_last (is_sprint_mem D p n npos rs)).2
 
 -- The sprint indicated by 'find_last_sprint_with_state' does
 -- in-fact contain the element 'rs'
 lemma last_sprint_with_state_is_sat (D : Devil) (p n : Nat)
-  (ppos : 0 < p) (npos : 0 < n) (rs : RunState) :
-  (∃ (i : Nat) (ilt : i < n), rs ∈ (make_run D p n ppos).sprints[i]'(by
+  (npos : 0 < n) (rs : RunState) :
+  (∃ (i : Nat) (ilt : i < n), rs ∈ (make_run D p n).sprints[i]'(by
     rwa [make_run_sprints_length])) →
-  rs ∈ (make_run D p n ppos).sprints[find_last_sprint_with_state D p n ppos npos rs]'(
-    last_sprint_with_state_lt_length D p n ppos npos rs
+  rs ∈ (make_run D p n).sprints[find_last_sprint_with_state D p n npos rs]'(
+    last_sprint_with_state_lt_length D p n npos rs
   ) := by
   rintro ⟨i, ilt, hmem⟩
   let i' : Fin (n - 1 + 1) := ⟨i, by rwa [(Nat.sub_one_add_one (Nat.ne_zero_of_lt npos))]⟩
-  exact _find_last_is_sat ((is_sprint_mem D p n ppos npos rs)) ⟨i', hmem⟩
+  exact _find_last_is_sat ((is_sprint_mem D p n npos rs)) ⟨i', hmem⟩
 
 -- If the devil is "nice", the runner will never visit a cell that was previously eaten.
 -- Note that this result is more general than 'make_run_journey_allowed_of_nice' in that
 -- it applies to *all* cells visited by the runner, not just those in the journey.
-lemma make_run_runner_avoids_eaten_cells_of_nice (D : Devil) (p n : Nat) (ppos : 0 < p) (hnice : nice D p) :
-  ∀ i (ilt : i < n) j (jlt : j < ((make_run D p n ppos).sprints[i]'(by
+lemma make_run_runner_avoids_eaten_cells_of_nice (D : Devil) (p n : Nat) (hnice : nice D p) :
+  ∀ i (ilt : i < n) j (jlt : j < ((make_run D p n).sprints[i]'(by
     rwa [make_run_sprints_length])).length) k (kle : k ≤ i),
-    (make_run D p n ppos).eaten[k]'(by
+    (make_run D p n).eaten[k]'(by
       rw [make_run_eaten_length]
       exact lt_trans (lt_of_le_of_lt kle ilt) (Nat.lt_add_one _)
-    ) ≠ loc (((make_run D p n ppos).sprints[i]'(by rwa [make_run_sprints_length]))[j]'(jlt)) := by
+    ) ≠ loc (((make_run D p n).sprints[i]'(by rwa [make_run_sprints_length]))[j]'(jlt)) := by
   intro i ilt j jlt k kle
-  rw [getElem_congr_coll (make_run_sprint D p n ppos i ilt)]
-  have lhs_rw : (make_run D p n ppos).eaten[k]'(by
+  rw [getElem_congr_coll (make_run_sprint D p n i ilt)]
+  have lhs_rw : (make_run D p n).eaten[k]'(by
     rw [make_run_eaten_length]
     exact lt_trans (lt_of_le_of_lt kle ilt) (Nat.lt_add_one _)
-  ) = ((make_run D p n ppos).eaten.take (i + 1))[k]'(by
+  ) = ((make_run D p n).eaten.take (i + 1))[k]'(by
     rw [List.length_take_of_le]
     · exact Nat.lt_add_one_of_le kle
     · rw [make_run_eaten_length]
@@ -921,18 +915,18 @@ lemma make_run_runner_avoids_eaten_cells_of_nice (D : Devil) (p n : Nat) (ppos :
   ) := by
     exact List.getElem_take.symm
   rw [lhs_rw]
-  rw [getElem_congr_coll (make_run_eaten_take D p i n ppos (lt_trans ilt (Nat.lt_add_one _)))]
+  rw [getElem_congr_coll (make_run_eaten_take D p i n (lt_trans ilt (Nat.lt_add_one _)))]
   intro h
-  rw [make_run_sprint D p n ppos i ilt] at jlt
-  let rs : RunState := (next_sprint (make_run D p i ppos))[j]'jlt
-  apply make_run_next_sprint_avoids_blocked_of_nice D p i ppos hnice rs (List.getElem_mem jlt)
+  rw [make_run_sprint D p n i ilt] at jlt
+  let rs : RunState := (next_sprint (make_run D p i))[j]'jlt
+  apply make_run_next_sprint_avoids_blocked_of_nice D p i hnice rs (List.getElem_mem jlt)
   apply List.mem_union_iff.mpr; left
   rw [← h]
   exact List.getElem_mem (by rw [make_run_eaten_length]; exact Nat.lt_add_one_of_le kle)
 
 -- If the devil is "nice", then no cell visited by the runner was ever eaten by the devil.
-lemma run_path_not_eaten_of_nice (D : Devil) (p n : Nat) (ppos : 0 < p) (hnice : nice D p) :
-  ∀ rs ∈ (RunPath D p n ppos), (loc rs) ∉ (make_run D p n ppos).eaten := by
+lemma run_path_not_eaten_of_nice (D : Devil) (p n : Nat) (hnice : nice D p) :
+  ∀ rs ∈ (RunPath D p n), (loc rs) ∉ (make_run D p n).eaten := by
   intro rs rsmem rseaten
   -- First handle the case where n = 0
   by_cases hnz : n = 0
@@ -947,9 +941,9 @@ lemma run_path_not_eaten_of_nice (D : Devil) (p n : Nat) (ppos : 0 < p) (hnice :
   have npos : 0 < n := Nat.pos_of_ne_zero hnnz
   -- Get the location of 'rs' within 'sprints'
   have mrsgEe_of_rpm :=
-    make_run_sprints_getElem_exists_of_run_path_mem D p n ppos npos rs rsmem
+    make_run_sprints_getElem_exists_of_run_path_mem D p n npos rs rsmem
   rcases mrsgEe_of_rpm with ⟨i, ilt, j, jlt, hij⟩
-  let MR : RunBuilder p := (make_run D p n ppos)
+  let MR : RunBuilder p := (make_run D p n)
   have snnil : MR.sprints ≠ [] := by
         apply List.ne_nil_of_length_pos
         rwa [make_run_sprints_length]
@@ -984,7 +978,7 @@ lemma run_path_not_eaten_of_nice (D : Devil) (p n : Nat) (ppos : 0 < p) (hnice :
   rename' hlast => hnl; push_neg at hnl
   -- If 'rs' wasn't eaten at the end, it must have
   -- been eaten in some shorter 'make_run'
-  have rseaten' : loc rs ∈ (make_run D p (n - 1) ppos).eaten := by
+  have rseaten' : loc rs ∈ (make_run D p (n - 1)).eaten := by
     rw [make_run_eaten_recurrence] at rseaten; swap
     · assumption
     rcases List.mem_append.mp rseaten with lhs | rhs
@@ -996,7 +990,7 @@ lemma run_path_not_eaten_of_nice (D : Devil) (p n : Nat) (ppos : 0 < p) (hnice :
     rw [make_run_eaten_length]; rfl
   -- Now, if the eaten cell was not visited in the last sprint, we can recurse
   by_cases hnmls : rs ∉ MR.sprints.getLast snnil
-  · apply run_path_not_eaten_of_nice D p (n - 1) ppos hnice rs _ rseaten'
+  · apply run_path_not_eaten_of_nice D p (n - 1) hnice rs _ rseaten'
     rw [run_path_recurrence] at rsmem; swap
     · assumption
     -- Lean weirdness work-around
