AngelDevil/Sprint.lean
@@ -6,39 +6,20 @@ import AngelDevil.Trace
 
 set_option linter.style.longLine false
 
--- A useful equivalence for the following definitions / lemmas
-lemma sprint_fin_prop (p : Nat) (start : RunState) (blocked : List (Int × Int)) (ppos : 0 < p) :
-  ∀ i, i < (trace (2 * p) start blocked).length ↔ i < 2 * p - 1 + 1 := by
-  intro i
-  constructor
-  · intro h
-    rw [Nat.sub_one_add_one]; swap
-    · apply Nat.ne_zero_of_lt
-      exact (Nat.mul_lt_mul_left (two_pos)).mpr ppos
-    rwa [trace_length] at h
-  · intro h
+abbrev sprint_end_fun (p : Nat) (start : RunState) (blocked : List (Int × Int)) :
+  Fin (2 * p + 1) → Prop := fun i ↦ ¬close p (loc start) (loc ((trace (2 * p + 1) start blocked)[i]'(by
     rw [trace_length]
-    rwa [Nat.sub_one_add_one] at h
-    apply Nat.ne_zero_iff_zero_lt.mpr
-    exact Nat.mul_pos two_pos ppos
-
-abbrev sprint_end_fun (p : Nat) (start : RunState) (blocked : List (Int × Int)) (ppos : 0 < p) :
-  Fin (2 * p - 1 + 1) → Prop := fun i ↦ ¬close p (loc start) (loc ((trace (2 * p) start blocked)[i]'(by
-    rw [sprint_fin_prop]
-    · exact i.2
-    · assumption
+    exact i.2
   )))
 
--- Define a "sprint" as the trace with length no greater than '2p' for which every
+-- Define a "sprint" as the trace with length no greater than '2p+1' for which every
 -- cell in the trace is "close" to the start.
+-- Note that the paper describes what I have formalized as a "sprint" as having cells
+-- v[0], v[1], v[2], ..., v[n], where n ≤ 2p. That means each sprint can have a maximum
+-- length of 2p + 1 (not just '2p', as I had mistakenly stated previously).
 def sprint (p : Nat) (start : RunState) (blocked : List (Int × Int)) : List RunState :=
-  trace (if h : (∃ rs : RunState, rs ∈ trace (2 * p) start blocked ∧ ¬close p (loc start) (loc rs)) then
-  (_find_first (sprint_end_fun p start blocked (by
-    rcases h with ⟨rs, h₀, h₁⟩
-    have ppos := List.length_pos_of_mem h₀
-    rw [trace_length] at ppos
-    exact Nat.pos_of_mul_pos_left ppos
-  ))) else (2 * p)) start blocked
+  trace (if (∃ rs : RunState, rs ∈ trace (2 * p + 1) start blocked ∧ ¬close p (loc start) (loc rs)) then
+  (_find_first (sprint_end_fun p start blocked)) else (2 * p + 1)) start blocked
 
 lemma sprint_getElem_zero_of_nonnil (p : Nat) (start : RunState) (blocked : List (Int × Int)) :
   (hnnil : sprint p start blocked ≠ []) →
@@ -48,62 +29,56 @@ lemma sprint_getElem_zero_of_nonnil (p : Nat) (start : RunState) (blocked : List
   apply trace_getElem_zero_of_nonnil
   exact hnnil
 
--- If 'p' is positive, the sprint will not be empty
-lemma sprint_nonnil_of_ppos (p : Nat) (start : RunState) (blocked : List (Int × Int)) :
-  0 < p → sprint p start blocked ≠ [] := by
-  intro ppos
-  apply List.ne_nil_of_length_pos
+lemma sprint_nonnil (p : Nat) (start : RunState) (blocked : List (Int × Int)) :
+  sprint p start blocked ≠ [] := by
+  apply List.ne_nil_of_length_pos (Nat.pos_of_ne_zero _)
   rw [sprint, trace_length]
   split_ifs with h
-  · rcases h with ⟨rs, h₀, h₁⟩
-    apply Nat.pos_of_ne_zero
+  · rcases h with ⟨rs, rsmem, hfar⟩
     intro hfind
-    have : sprint_end_fun p start blocked ppos 0 := by
+    have : sprint_end_fun p start blocked 0 := by
       rw [← Fin.val_eq_zero_iff.mp hfind]
       apply _find_first_is_sat
-      rcases List.getElem_of_mem h₀ with ⟨i, ilt, hirs⟩
-      let i' : Fin (2 * p - 1 + 1) := ⟨i, (sprint_fin_prop p start blocked ppos i).mp ilt⟩
+      rcases List.getElem_of_mem rsmem with ⟨i, ilt, hirs⟩
+      let i' : Fin (2 * p + 1) := ⟨i, by rwa [trace_length] at ilt⟩
       use i'
       unfold sprint_end_fun
-      rw [← hirs] at h₁
-      exact h₁
+      rw [← hirs] at hfar
+      exact hfar
     apply this
-    convert close_self p (loc start)
+    convert close_self _ _
     apply trace_getElem_zero_of_nonnil
     apply List.ne_nil_of_length_pos
     rw [trace_length]
-    exact Nat.mul_pos two_pos ppos
-  exact Nat.mul_pos (by norm_num) ppos
+    exact Nat.add_one_pos _
+  · exact Nat.add_one_ne_zero _
 
-lemma sprint_getElem_zero_of_ppos (p : Nat) (start : RunState) (blocked : List (Int × Int)) :
-  (ppos : 0 < p) → (sprint p start blocked)[0]'(by
+lemma sprint_getElem_zero (p : Nat) (start : RunState) (blocked : List (Int × Int)) :
+  (sprint p start blocked)[0]'(by
     apply List.length_pos_of_ne_nil
-    exact sprint_nonnil_of_ppos p start blocked ppos
+    exact sprint_nonnil p start blocked
   ) = start :=
-  fun ppos ↦
-  sprint_getElem_zero_of_nonnil p start blocked (sprint_nonnil_of_ppos p start blocked ppos)
+  sprint_getElem_zero_of_nonnil p start blocked (sprint_nonnil p start blocked)
 
--- The maximum sprint length is 2 * p
+-- The maximum sprint length is 2 * p + 1
 lemma sprint_length_le (p : Nat) (start : RunState) (blocked : List (Int × Int)) :
-  (sprint p start blocked).length ≤ 2 * p := by
+  (sprint p start blocked).length ≤ 2 * p + 1 := by
   unfold sprint
   rw [trace_length]
   split_ifs with h; swap
-  · rfl
+  · exact le_refl _
   rcases h with ⟨rs, hmem, hnclose⟩
   rcases List.getElem_of_mem hmem with ⟨i, ilt, hirs⟩
   apply le_of_lt (lt_of_lt_of_le (Fin.prop _) _)
-  rw [Nat.sub_one_add_one]
-  rw [trace_length] at ilt
-  apply Nat.ne_zero_of_lt ilt
+  exact le_refl _
 
 -- The minimum sprint length is p+1
-lemma sprint_length_lb (p : Nat) (start : RunState) (blocked : List (Int × Int)) (ppos : 0 < p) :
+lemma sprint_length_lb (p : Nat) (start : RunState) (blocked : List (Int × Int)) :
   p < (sprint p start blocked).length := by
   unfold sprint
   -- This hypothesis is easier to work with than the final goal
-  have : ∀ (i : Fin (2 * p - 1 + 1)), i.val ≤ p →
-    ¬sprint_end_fun p start blocked ppos i := by
+  have : ∀ (i : Fin (2 * p + 1)), i.val ≤ p →
+    ¬sprint_end_fun p start blocked i := by
     intro i ile
     unfold sprint_end_fun; push_neg
     rw [Fin.getElem_fin, trace_getElem_getLast]
@@ -116,12 +91,9 @@ lemma sprint_length_lb (p : Nat) (start : RunState) (blocked : List (Int × Int)
     apply _find_first_is_sat
     rcases h with ⟨rs, rsmem, h⟩
     rcases List.getElem_of_mem rsmem with ⟨i, ilt, hirs⟩
-    have ilt' : i < 2 * p - 1 + 1 := by
-      rw [trace_length] at ilt
-      rwa [Nat.sub_one_add_one]
-      apply Nat.mul_ne_zero (by norm_num)
-      exact Nat.ne_zero_of_lt ppos
-    let i' : Fin (2 * p - 1 + 1) := ⟨i, ilt'⟩
+    have ilt' : i < 2 * p + 1 := by
+      rwa [trace_length] at ilt
+    let i' : Fin (2 * p + 1) := ⟨i, ilt'⟩
     use i'
     convert h
   · linarith
@@ -129,27 +101,25 @@ lemma sprint_length_lb (p : Nat) (start : RunState) (blocked : List (Int × Int)
 -- Each run state in a sprint is equal to the corresponding element of the corresponding trace
 lemma sprint_getElem_eq_trace_getElem (p : Nat) (start : RunState) (blocked : List (Int × Int)) :
   ∀ i (ilt : i < (sprint p start blocked).length),
-  (sprint p start blocked)[i] = (trace (2 * p) start blocked)[i]'(by
+  (sprint p start blocked)[i] = (trace (2 * p + 1) start blocked)[i]'(by
     rw [trace_length]
     exact lt_of_lt_of_le ilt (sprint_length_le p start blocked)
   ) := by
   intro i ilt
-  have twoppos : 0 < (2 * p) := by
+  have twoppos : 0 < (2 * p + 1) := by
     apply lt_of_le_of_lt (Nat.zero_le _)
     exact (lt_of_lt_of_le ilt (sprint_length_le p start blocked))
   unfold sprint
   split_ifs with h
-  · rw [getElem_congr_coll (trace_take (2 * p) start blocked _ _)]; swap
-    · apply le_of_lt
-      nth_rw 14 [← Nat.sub_one_add_one (Nat.ne_zero_of_lt twoppos)]
-      exact Fin.prop _
+  · rw [getElem_congr_coll (trace_take (2 * p + 1) start blocked _ _)]; swap
+    · exact le_of_lt (Fin.prop _)
     apply List.getElem_take
   rfl
 
 -- All run states in a sprint are close to the start of that sprint
-lemma sprint_close_mem_head (p : Nat) (ppos : 0 < p) (start : RunState) (blocked : List (Int × Int)) :
+lemma sprint_close_mem_head (p : Nat) (start : RunState) (blocked : List (Int × Int)) :
   ∀ x ∈ (sprint p start blocked), close p (loc x)
-  (loc ((sprint p start blocked).head (sprint_nonnil_of_ppos p start blocked ppos))) := by
+  (loc ((sprint p start blocked).head (sprint_nonnil p start blocked))) := by
   intro x hmem
   rw [← List.getElem_zero_eq_head]; swap
   · exact List.length_pos_of_mem hmem
@@ -159,27 +129,23 @@ lemma sprint_close_mem_head (p : Nat) (ppos : 0 < p) (start : RunState) (blocked
   rw [sprint_getElem_eq_trace_getElem p start blocked i ilt]
   by_contra! h
   have ilt' := lt_of_lt_of_le ilt (sprint_length_le p start blocked)
-  have ppos : 0 < p := by
-    apply (Nat.mul_lt_mul_left (two_pos)).mp
-    rw [mul_zero]
-    exact lt_of_le_of_lt (Nat.zero_le _) ilt'
-  let i' : Fin (2 * p - 1 + 1) := ⟨i, lt_of_lt_of_eq ilt' (Nat.sub_one_add_one (Nat.ne_zero_of_lt ilt')).symm⟩
+  let i' : Fin (2 * p + 1) := ⟨i, lt_of_lt_of_eq ilt' (Nat.sub_one_add_one (Nat.ne_zero_of_lt ilt')).symm⟩
   unfold sprint at ilt
-  have hthen : ∃ rs ∈ trace (2 * p) start blocked, ¬close p (loc start) (loc rs) := by
-    use (trace (2 * p) start blocked)[i]'(by rwa [trace_length])
+  have hthen : ∃ rs ∈ trace (2 * p + 1) start blocked, ¬close p (loc start) (loc rs) := by
+    use (trace (2 * p + 1) start blocked)[i]'(by rwa [trace_length])
     use List.getElem_mem (by rwa [trace_length])
-  rw [dif_pos hthen, trace_length] at ilt
-  have := _find_first_is_first (sprint_end_fun p start blocked ppos) i' h
+  rw [if_pos hthen, trace_length] at ilt
+  have := _find_first_is_first (sprint_end_fun p start blocked) i' h
   exact Nat.not_lt.mpr this ilt
 
 -- Prove that the first and last cells in a sprint are "close"
-lemma sprint_close_first_last (p : Nat) (hpos : 0 < p) (start : RunState) (blocked : List (Int × Int)) :
+lemma sprint_close_first_last (p : Nat) (start : RunState) (blocked : List (Int × Int)) :
   close p
-  (loc ((sprint p start blocked).head (sprint_nonnil_of_ppos p start blocked hpos)))
-  (loc ((sprint p start blocked).getLast (sprint_nonnil_of_ppos p start blocked hpos))) := by
-  have hnnil := sprint_nonnil_of_ppos p start blocked hpos
+  (loc ((sprint p start blocked).head (sprint_nonnil p start blocked)))
+  (loc ((sprint p start blocked).getLast (sprint_nonnil p start blocked))) := by
+  have hnnil := sprint_nonnil p start blocked
   rw [close_comm]
-  exact sprint_close_mem_head p hpos start blocked _ (List.getLast_mem hnnil)
+  exact sprint_close_mem_head p start blocked _ (List.getLast_mem hnnil)
 
 -- The runner never visits an eaten cell
 -- (as long as they don't start on an eaten cell)
